finished the refinement of map_var_bit_to_var_acc, and refined the previous proofs of push_on_stack

Cook_Levin/IMP-_To_SAS+/IMP-_To_IMP--/IMP_Minus_To_IMP_Minus_Minus_IMP.thy
@@ -18,6 +18,293 @@ subsection \<open>Useful Definitions and Lemmas\<close>
 
 subsection \<open>map_var_bit_to_var\<close>
 
+subsubsection \<open>map_var_bit_to_var_aux\<close>
+
+fun map_var_bit_to_var_aux :: "nat \<Rightarrow> nat \<Rightarrow> nat \<Rightarrow> nat" where 
+"map_var_bit_to_var_aux acc v n = ((var_bit_to_var_nat (prod_encode (v,hd_nat n)))## acc)"
+
+record map_var_bit_to_var_aux_state =
+  map_var_bit_to_var_aux_acc::nat
+  map_var_bit_to_var_aux_v::nat
+  map_var_bit_to_var_aux_n::nat
+  map_var_bit_to_var_aux_ret::nat
+
+abbreviation "map_var_bit_to_var_aux_prefix \<equiv> ''map_var_bit_to_var_aux.''"
+abbreviation "map_var_bit_to_var_aux_acc_str \<equiv> ''acc''"
+abbreviation "map_var_bit_to_var_aux_v_str \<equiv> ''v''"
+abbreviation "map_var_bit_to_var_aux_n_str \<equiv> ''n''"
+abbreviation "map_var_bit_to_var_aux_ret_str \<equiv> ''ret''"
+
+
+function map_var_bit_to_var_aux_imp :: "map_var_bit_to_var_aux_state \<Rightarrow> map_var_bit_to_var_aux_state" where 
+"map_var_bit_to_var_aux_imp s = 
+(let
+    hd_xs' = map_var_bit_to_var_aux_n s;
+    hd_ret' = 0;
+    hd_state = \<lparr>hd_xs = hd_xs',
+                hd_ret = hd_ret'\<rparr>;
+    hd_ret_state = hd_imp hd_state;
+
+    prod_encode_a' = map_var_bit_to_var_aux_v s;
+    prod_encode_b' = hd_ret hd_ret_state;
+    prod_encode_ret' = 0;
+    prod_encode_state = \<lparr>prod_encode_a = prod_encode_a',
+                         prod_encode_b = prod_encode_b',
+                         prod_encode_ret = prod_encode_ret'\<rparr>;
+    prod_encode_ret_state = prod_encode_imp prod_encode_state;
+
+    var_bit_to_var_nat_n' = prod_encode_ret prod_encode_ret_state;
+    var_bit_to_var_nat_ret' = 0;
+    var_bit_to_var_nat_state = \<lparr>var_bit_to_var_nat_n = var_bit_to_var_nat_n',
+                                var_bit_to_var_nat_ret = var_bit_to_var_nat_ret'\<rparr>;
+    var_bit_to_var_nat_ret_state = var_bit_to_var_nat_imp var_bit_to_var_nat_state;
+
+    cons_h' = var_bit_to_var_nat_ret var_bit_to_var_nat_ret_state;
+    cons_t' = map_var_bit_to_var_aux_acc s;
+    cons_ret' = 0;
+    cons_state = \<lparr>cons_h = cons_h',
+                  cons_t = cons_t', 
+                  cons_ret = cons_ret'\<rparr>;
+    cons_ret_state = cons_imp cons_state;
+    map_var_bit_to_var_aux_ret' = cons_ret cons_ret_state;
+    
+    tl_xs' = map_var_bit_to_var_aux_n s;
+    tl_ret' = 0;
+    tl_state = \<lparr>tl_xs = tl_xs', 
+                tl_ret = tl_ret'\<rparr>;
+    tl_ret_state = tl_imp tl_state;
+
+    map_var_bit_to_var_aux_n' = tl_ret tl_ret_state;
+    ret = \<lparr>map_var_bit_to_var_aux_acc = map_var_bit_to_var_aux_acc s,
+          map_var_bit_to_var_aux_v = map_var_bit_to_var_aux_v s,
+          map_var_bit_to_var_aux_n = map_var_bit_to_var_aux_n',
+          map_var_bit_to_var_aux_ret = map_var_bit_to_var_aux_ret'\<rparr>
+    in
+     ret)
+    " by simp+
+    termination
+    apply (relation "measure map_var_bit_to_var_aux_acc")
+    apply simp 
+    done 
+
+declare map_var_bit_to_var_aux_imp.simps[simp del]
+
+lemma map_var_bit_to_var_aux_imp_correct[let_function_correctness]:
+"map_var_bit_to_var_aux_ret (map_var_bit_to_var_aux_imp s) = 
+  map_var_bit_to_var_aux (map_var_bit_to_var_aux_acc s) (map_var_bit_to_var_aux_v s) (map_var_bit_to_var_aux_n s)
+  \<and> map_var_bit_to_var_aux_n (map_var_bit_to_var_aux_imp s) = tl_nat (map_var_bit_to_var_aux_n s)"
+apply (subst map_var_bit_to_var_aux_imp.simps)+
+apply (auto simp add: hd_imp_correct prod_encode_imp_correct var_bit_to_var_nat_imp_correct cons_imp_correct
+  tl_imp_correct)
+done 
+
+function map_var_bit_to_var_aux_imp_time :: "nat \<Rightarrow> map_var_bit_to_var_aux_state \<Rightarrow> nat" where 
+"map_var_bit_to_var_aux_imp_time t s = 
+(let
+    hd_xs' = map_var_bit_to_var_aux_n s;
+    t = t + 2;
+    hd_ret' = 0;
+    t = t + 2;
+    hd_state = \<lparr>hd_xs = hd_xs',
+                hd_ret = hd_ret'\<rparr>;
+    hd_ret_state = hd_imp hd_state;
+    t = t + hd_imp_time 0 hd_state;
+
+    prod_encode_a' = map_var_bit_to_var_aux_v s;
+    t = t + 2;
+    prod_encode_b' = hd_ret hd_ret_state;
+    t = t + 2;
+    prod_encode_ret' = 0;
+    t = t + 2;
+    prod_encode_state = \<lparr>prod_encode_a = prod_encode_a',
+                         prod_encode_b = prod_encode_b',
+                         prod_encode_ret = prod_encode_ret'\<rparr>;
+    prod_encode_ret_state = prod_encode_imp prod_encode_state;
+    t = t + prod_encode_imp_time 0 prod_encode_state;
+
+    var_bit_to_var_nat_n' = prod_encode_ret prod_encode_ret_state;
+    t = t + 2;
+    var_bit_to_var_nat_ret' = 0;
+    t = t + 2;
+    var_bit_to_var_nat_state = \<lparr>var_bit_to_var_nat_n = var_bit_to_var_nat_n',
+                                var_bit_to_var_nat_ret = var_bit_to_var_nat_ret'\<rparr>;
+    var_bit_to_var_nat_ret_state = var_bit_to_var_nat_imp var_bit_to_var_nat_state;
+    t = t + var_bit_to_var_nat_imp_time 0 var_bit_to_var_nat_state;
+
+    cons_h' = var_bit_to_var_nat_ret var_bit_to_var_nat_ret_state;
+    t = t + 2;
+    cons_t' = map_var_bit_to_var_aux_acc s;
+    t = t + 2;
+    cons_ret' = 0;
+    t = t + 2;
+    cons_state = \<lparr>cons_h = cons_h',
+                  cons_t = cons_t', 
+                  cons_ret = cons_ret'\<rparr>;
+    cons_ret_state = cons_imp cons_state;
+    t = t + cons_imp_time 0 cons_state;
+    map_var_bit_to_var_aux_ret' = cons_ret cons_ret_state;
+    t = t + 2;
+
+    tl_xs' = map_var_bit_to_var_aux_n s;
+    t = t + 2;
+    tl_ret' = 0;
+    t = t + 2;
+    tl_state = \<lparr>tl_xs = tl_xs', 
+                tl_ret = tl_ret'\<rparr>;
+    tl_ret_state = tl_imp tl_state;
+    t = t + tl_imp_time 0 tl_state;
+
+    map_var_bit_to_var_aux_n' = tl_ret tl_ret_state;
+    t = t + 2;
+    ret = \<lparr>map_var_bit_to_var_aux_acc = map_var_bit_to_var_aux_acc s,
+          map_var_bit_to_var_aux_v = map_var_bit_to_var_aux_v s,
+          map_var_bit_to_var_aux_n = map_var_bit_to_var_aux_n',
+          map_var_bit_to_var_aux_ret = map_var_bit_to_var_aux_ret'\<rparr>
+    in
+     t)
+    " by auto
+    termination
+    apply (relation "measure (map_var_bit_to_var_aux_acc \<circ> snd)")
+    apply simp 
+    done 
+
+declare map_var_bit_to_var_aux_imp_time.simps[simp del]
+
+definition  "map_var_bit_to_var_aux_IMP_Minus \<equiv> 
+  (hd_prefix @ hd_xs_str) ::= (A (V map_var_bit_to_var_aux_n_str));;
+  (hd_prefix @ hd_ret_str) ::= (A (N 0));;
+  invoke_subprogram hd_prefix hd_IMP_Minus;;
+
+  (prod_encode_prefix @ prod_encode_a_str) ::= (A (V map_var_bit_to_var_aux_v_str));;
+  (prod_encode_prefix @ prod_encode_b_str) ::= (A (V (hd_prefix @ hd_ret_str)));;
+  (prod_encode_prefix @ prod_encode_ret_str) ::= (A (N 0));;
+  invoke_subprogram prod_encode_prefix prod_encode_IMP_Minus;;
+
+  (var_bit_to_var_nat_prefix @ var_bit_to_var_nat_n_str) ::= (A (V (prod_encode_prefix @ prod_encode_ret_str)));;
+  (var_bit_to_var_nat_prefix @ var_bit_to_var_nat_ret_str) ::= (A (N 0));;
+  invoke_subprogram var_bit_to_var_nat_prefix var_bit_to_var_nat_IMP_Minus;;
+
+  (cons_prefix @ cons_h_str) ::= (A (V (var_bit_to_var_nat_prefix @ var_bit_to_var_nat_ret_str)));;
+  (cons_prefix @ cons_t_str) ::= (A (V map_var_bit_to_var_aux_acc_str));;
+  (cons_prefix @ cons_ret_str) ::= (A (N 0));;
+  invoke_subprogram cons_prefix cons_IMP_Minus;;
+  map_var_bit_to_var_aux_ret_str ::= (A (V (cons_prefix @ cons_ret_str)));;
+
+  (tl_prefix @ tl_xs_str) ::= (A (V map_var_bit_to_var_aux_n_str));;
+  (tl_prefix @ tl_ret_str) ::= (A (N 0));;
+  invoke_subprogram tl_prefix tl_IMP_Minus;;
+
+  map_var_bit_to_var_aux_n_str ::= (A (V (tl_prefix @ tl_ret_str)))
+"
+
+definition "map_var_bit_to_var_aux_imp_to_HOL_state p s =
+  \<lparr>map_var_bit_to_var_aux_acc = (s (add_prefix p map_var_bit_to_var_aux_acc_str)),
+  map_var_bit_to_var_aux_v = (s (add_prefix p map_var_bit_to_var_aux_v_str)),
+  map_var_bit_to_var_aux_n = (s (add_prefix p map_var_bit_to_var_aux_n_str)),
+  map_var_bit_to_var_aux_ret = (s (add_prefix p map_var_bit_to_var_aux_ret_str))\<rparr>"
+
+lemmas map_var_bit_to_var_aux_state_translators =
+  map_var_bit_to_var_aux_imp_to_HOL_state_def
+  hd_imp_to_HOL_state_def
+  prod_encode_imp_to_HOL_state_def
+  var_bit_to_var_nat_imp_to_HOL_state_def
+  cons_imp_to_HOL_state_def
+  tl_imp_to_HOL_state_def
+
+abbreviation "map_var_bit_to_var_aux_IMP_vars \<equiv> {
+  map_var_bit_to_var_aux_acc_str, map_var_bit_to_var_aux_v_str, 
+  map_var_bit_to_var_aux_n_str, map_var_bit_to_var_aux_ret_str}"
+
+lemma map_var_bit_to_var_aux_IMP_Minus_correct_function_ret:
+  "(invoke_subprogram p map_var_bit_to_var_aux_IMP_Minus, s) \<Rightarrow>\<^bsup>t\<^esup> s' \<Longrightarrow>
+     s' (add_prefix p map_var_bit_to_var_aux_ret_str)
+      = map_var_bit_to_var_aux_ret
+          (map_var_bit_to_var_aux_imp (map_var_bit_to_var_aux_imp_to_HOL_state p s))"
+apply (simp only: map_var_bit_to_var_aux_IMP_Minus_def prefix_simps)
+apply (erule Seq_E)+
+apply (erule  hd_IMP_Minus_correct[where vars=map_var_bit_to_var_aux_IMP_vars])
+subgoal premises p using p(19) by fastforce
+apply (erule  prod_encode_IMP_Minus_correct[where vars=map_var_bit_to_var_aux_IMP_vars])
+subgoal premises p using p(21) by fastforce
+apply (erule  var_bit_to_var_nat_IMP_Minus_correct[where vars=map_var_bit_to_var_aux_IMP_vars])
+subgoal premises p using p(23) by fastforce
+apply (erule  cons_IMP_Minus_correct[where vars=map_var_bit_to_var_aux_IMP_vars])
+subgoal premises p using p(25) by fastforce
+apply (erule  tl_IMP_Minus_correct[where vars="map_var_bit_to_var_aux_IMP_vars"])
+subgoal premises p using p(27) by fastforce
+apply (clarsimp simp add:
+  map_var_bit_to_var_aux_state_translators Let_def map_var_bit_to_var_aux_imp.simps)
+subgoal premises p
+  using p(10) p(8) p(6) p(4) p(2) by force 
+done 
+
+lemma map_var_bit_to_var_aux_IMP_Minus_correct_function_n:
+  "(invoke_subprogram p map_var_bit_to_var_aux_IMP_Minus, s) \<Rightarrow>\<^bsup>t\<^esup> s' \<Longrightarrow>
+     s' (add_prefix p map_var_bit_to_var_aux_n_str)
+      = map_var_bit_to_var_aux_n
+          (map_var_bit_to_var_aux_imp (map_var_bit_to_var_aux_imp_to_HOL_state p s))"
+apply (simp only: map_var_bit_to_var_aux_IMP_Minus_def prefix_simps)
+apply (erule Seq_E)+
+apply (erule  hd_IMP_Minus_correct[where vars=map_var_bit_to_var_aux_IMP_vars])
+subgoal premises p using p(19) by fastforce
+apply (erule  prod_encode_IMP_Minus_correct[where vars=map_var_bit_to_var_aux_IMP_vars])
+subgoal premises p using p(21) by fastforce
+apply (erule  var_bit_to_var_nat_IMP_Minus_correct[where vars=map_var_bit_to_var_aux_IMP_vars])
+subgoal premises p using p(23) by fastforce
+apply (erule  cons_IMP_Minus_correct[where vars=map_var_bit_to_var_aux_IMP_vars])
+subgoal premises p using p(25) by fastforce
+apply (erule  tl_IMP_Minus_correct[where vars="map_var_bit_to_var_aux_IMP_vars"])
+subgoal premises p using p(27) by fastforce
+apply (clarsimp simp add:
+  map_var_bit_to_var_aux_state_translators Let_def map_var_bit_to_var_aux_imp.simps)
+subgoal premises p
+  using p(10) p(8) p(6) p(4) p(2) by force 
+done 
+
+lemma map_var_bit_to_var_aux_IMP_Minus_correct_effects:
+  "\<lbrakk>(invoke_subprogram (p @ map_var_bit_to_var_aux_pref) map_var_bit_to_var_aux_IMP_Minus, s) \<Rightarrow>\<^bsup>t\<^esup> s';
+    v \<in> vars; \<not> (prefix map_var_bit_to_var_aux_pref v)\<rbrakk>
+   \<Longrightarrow> s (add_prefix p v) = s' (add_prefix p v)"
+  using com_add_prefix_valid'' com_only_vars prefix_def
+  by blast            
+
+
+lemma map_var_bit_to_var_aux_IMP_Minus_correct_time:
+  "(invoke_subprogram p map_var_bit_to_var_aux_IMP_Minus, s) \<Rightarrow>\<^bsup>t\<^esup> s' \<Longrightarrow>
+     t = map_var_bit_to_var_aux_imp_time 0 (map_var_bit_to_var_aux_imp_to_HOL_state p s)"
+apply (simp only: map_var_bit_to_var_aux_IMP_Minus_def prefix_simps)
+apply (erule Seq_tE)+
+apply (erule hd_IMP_Minus_correct[where vars=map_var_bit_to_var_aux_IMP_vars])
+subgoal premises p using p(37) by fastforce
+apply (erule prod_encode_IMP_Minus_correct[where vars=map_var_bit_to_var_aux_IMP_vars])
+subgoal premises p using p(39) by fastforce
+apply (erule var_bit_to_var_nat_IMP_Minus_correct[where vars=map_var_bit_to_var_aux_IMP_vars])
+subgoal premises p using p(41) by fastforce
+apply (erule cons_IMP_Minus_correct[where vars=map_var_bit_to_var_aux_IMP_vars])
+subgoal premises p using p(43) by fastforce
+apply (erule tl_IMP_Minus_correct[where vars=map_var_bit_to_var_aux_IMP_vars])
+subgoal premises p using p(45) by fastforce
+apply (force simp: map_var_bit_to_var_aux_imp_time.simps 
+  Let_def map_var_bit_to_var_aux_state_translators)
+done 
+
+lemma map_var_bit_to_var_aux_IMP_Minus_correct[functional_correctness]:
+  "\<lbrakk>(invoke_subprogram (p1 @ p2) map_var_bit_to_var_aux_IMP_Minus, s) \<Rightarrow>\<^bsup>t\<^esup> s';
+    \<And>v. v \<in> vars \<Longrightarrow> \<not> (set p2 \<subseteq> set v);
+    \<lbrakk>t = (map_var_bit_to_var_aux_imp_time 0 (map_var_bit_to_var_aux_imp_to_HOL_state (p1 @ p2) s));
+     s' (add_prefix (p1 @ p2) map_var_bit_to_var_aux_ret_str) =
+          map_var_bit_to_var_aux_ret (map_var_bit_to_var_aux_imp
+                                        (map_var_bit_to_var_aux_imp_to_HOL_state (p1 @ p2) s));
+     s' (add_prefix (p1 @ p2) map_var_bit_to_var_aux_n_str) =
+          map_var_bit_to_var_aux_n (map_var_bit_to_var_aux_imp
+                                        (map_var_bit_to_var_aux_imp_to_HOL_state (p1 @ p2) s));
+     \<And>v. v \<in> vars \<Longrightarrow> s (add_prefix p1 v) = s' (add_prefix p1 v)\<rbrakk>
+   \<Longrightarrow> P\<rbrakk> \<Longrightarrow> P"
+  using map_var_bit_to_var_aux_IMP_Minus_correct_function_ret 
+  map_var_bit_to_var_aux_IMP_Minus_correct_function_n
+  by (auto simp: map_var_bit_to_var_aux_IMP_Minus_correct_time)
+    (meson map_var_bit_to_var_aux_IMP_Minus_correct_effects set_mono_prefix) 
+
 subsubsection \<open>map_var_bit_to_var_acc\<close>
 
 fun map_var_bit_to_var_acc' :: "nat \<Rightarrow> nat \<Rightarrow> nat \<Rightarrow> nat" where 
@@ -52,48 +339,25 @@ abbreviation "map_var_bit_to_var_acc_ret_str \<equiv> ''ret''"
 
 definition "map_var_bit_to_var_acc_state_upd s \<equiv>
   let
-    hd_xs' = map_var_bit_to_var_acc_n s;
-    hd_ret' = 0;
-    hd_state = \<lparr>hd_xs = hd_xs',
-                hd_ret = hd_ret'\<rparr>;
-    hd_ret_state = hd_imp hd_state;
-    hd_result = hd_ret hd_ret_state;
-    prod_encode_a' = map_var_bit_to_var_acc_v s;
-    prod_encode_b' = hd_result;
-    prod_encode_ret' = 0;
-    prod_encode_state = \<lparr>prod_encode_a = prod_encode_a',
-                         prod_encode_b = prod_encode_b',
-      prod_encode_ret = prod_encode_ret'\<rparr>;
-    prod_encode_ret_state = prod_encode_imp prod_encode_state;
-    prod_encode_result = prod_encode_ret prod_encode_ret_state;
-    var_bit_to_var_nat_n' = prod_encode_result;
-    var_bit_to_var_nat_ret' = 0;
-    var_bit_to_var_nat_state = \<lparr>var_bit_to_var_nat_n = var_bit_to_var_nat_n',
-                                var_bit_to_var_nat_ret = var_bit_to_var_nat_ret'\<rparr>;
-    var_bit_to_var_nat_ret_state = var_bit_to_var_nat_imp var_bit_to_var_nat_state;
-    var_bit_to_var_nat_result = var_bit_to_var_nat_ret var_bit_to_var_nat_ret_state;
-    cons_h' = var_bit_to_var_nat_result;
-    cons_t' = map_var_bit_to_var_acc_acc s;
-    cons_ret' = 0;
-    cons_state = \<lparr>cons_h = cons_h',
-                  cons_t = cons_t', 
-                  cons_ret = cons_ret'\<rparr>;
-    cons_ret_state = cons_imp cons_state;
-    cons_result = cons_ret cons_ret_state;
-    tl_xs' = map_var_bit_to_var_acc_n s;
-    tl_ret' = 0;
-    tl_state = \<lparr>tl_xs = tl_xs', 
-                tl_ret = tl_ret'\<rparr>;
-    tl_ret_state = tl_imp tl_state;
-    tl_result = tl_ret tl_ret_state;
-    map_var_bit_to_var_acc_acc' = cons_result;
-    map_var_bit_to_var_acc_v' = map_var_bit_to_var_acc_v s;
-    map_var_bit_to_var_acc_n' = tl_result;
-    map_var_bit_to_var_acc_ret' = map_var_bit_to_var_acc_ret s;
+    map_var_bit_to_var_aux_acc' = map_var_bit_to_var_acc_acc s;
+    map_var_bit_to_var_aux_v' = map_var_bit_to_var_acc_v s;
+    map_var_bit_to_var_aux_n' = map_var_bit_to_var_acc_n s;
+    map_var_bit_to_var_aux_ret' = 0;
+    map_var_bit_to_var_aux_state = 
+      \<lparr>map_var_bit_to_var_aux_acc = map_var_bit_to_var_aux_acc',
+      map_var_bit_to_var_aux_v = map_var_bit_to_var_aux_v',
+      map_var_bit_to_var_aux_n = map_var_bit_to_var_aux_n',
+      map_var_bit_to_var_aux_ret = map_var_bit_to_var_aux_ret'\<rparr>;
+    map_var_bit_to_var_aux_ret_state = 
+        map_var_bit_to_var_aux_imp map_var_bit_to_var_aux_state;
+
+
+    map_var_bit_to_var_acc_acc' = map_var_bit_to_var_aux_ret map_var_bit_to_var_aux_ret_state;
+    map_var_bit_to_var_acc_n' = map_var_bit_to_var_aux_n map_var_bit_to_var_aux_ret_state;
     ret = \<lparr>map_var_bit_to_var_acc_acc = map_var_bit_to_var_acc_acc',
-           map_var_bit_to_var_acc_v = map_var_bit_to_var_acc_v',
+           map_var_bit_to_var_acc_v = map_var_bit_to_var_acc_v s,
            map_var_bit_to_var_acc_n = map_var_bit_to_var_acc_n',
-           map_var_bit_to_var_acc_ret = map_var_bit_to_var_acc_ret'\<rparr>
+           map_var_bit_to_var_acc_ret = map_var_bit_to_var_acc_ret s\<rparr>
     in ret
 "
 
@@ -106,13 +370,10 @@ definition "map_var_bit_to_var_acc_imp_compute_loop_condition s \<equiv>
 
 definition "map_var_bit_to_var_acc_imp_after_loop s \<equiv>
   (let
-    map_var_bit_to_var_acc_acc' = map_var_bit_to_var_acc_acc s;
-    map_var_bit_to_var_acc_v' = map_var_bit_to_var_acc_v s;
-    map_var_bit_to_var_acc_n' = map_var_bit_to_var_acc_n s;
     map_var_bit_to_var_acc_ret' = map_var_bit_to_var_acc_acc s;
-    ret = \<lparr>map_var_bit_to_var_acc_acc = map_var_bit_to_var_acc_acc',
-           map_var_bit_to_var_acc_v = map_var_bit_to_var_acc_v',
-           map_var_bit_to_var_acc_n = map_var_bit_to_var_acc_n',
+    ret = \<lparr>map_var_bit_to_var_acc_acc = map_var_bit_to_var_acc_acc s,
+           map_var_bit_to_var_acc_v = map_var_bit_to_var_acc_v s,
+           map_var_bit_to_var_acc_n = map_var_bit_to_var_acc_n s,
            map_var_bit_to_var_acc_ret = map_var_bit_to_var_acc_ret'\<rparr>
    in ret
   )"
@@ -136,7 +397,8 @@ function map_var_bit_to_var_acc_imp::
   by simp+
 termination 
   apply (relation "measure map_var_bit_to_var_acc_n")
-   apply (simp add: map_var_bit_to_var_acc_imp_subprogram_simps tl_imp_correct)+
+   apply (simp add: map_var_bit_to_var_acc_imp_subprogram_simps 
+      map_var_bit_to_var_aux_imp_correct Let_def)+
   done
 
 declare map_var_bit_to_var_acc_imp.simps [simp del]
@@ -151,80 +413,36 @@ lemma map_var_bit_to_var_acc_imp_correct[let_function_correctness]:
   apply (simp del: map_var_bit_to_var_acc'.simps 
               add: map_var_bit_to_var_acc_imp_subprogram_simps Let_def 
                    fst_nat_fst'_nat snd_nat_snd'_nat snd'_imp_correct fst'_imp_correct
-                   hd_imp_correct prod_encode_imp_correct var_bit_to_var_nat_imp_correct
-                   cons_imp_correct tl_imp_correct)
+                   map_var_bit_to_var_aux_imp_correct tl_imp_correct)
   done            
 
 definition "map_var_bit_to_var_acc_state_upd_time t s \<equiv>
   let
-    hd_xs' = map_var_bit_to_var_acc_n s;
+    map_var_bit_to_var_aux_acc' = map_var_bit_to_var_acc_acc s;
     t = t + 2;
-    hd_ret' = 0;
+    map_var_bit_to_var_aux_v' = map_var_bit_to_var_acc_v s;
     t = t + 2;
-    hd_state = \<lparr>hd_xs = hd_xs',
-                hd_ret = hd_ret'\<rparr>;
-    hd_ret_state = hd_imp hd_state;
-    t = t + hd_imp_time 0 hd_state;
-    hd_result = hd_ret hd_ret_state;
+    map_var_bit_to_var_aux_n' = map_var_bit_to_var_acc_n s;
     t = t + 2;
-    prod_encode_a' = map_var_bit_to_var_acc_v s;
+    map_var_bit_to_var_aux_ret' = 0;
     t = t + 2;
-    prod_encode_b' = hd_result;
+    map_var_bit_to_var_aux_state = 
+      \<lparr>map_var_bit_to_var_aux_acc = map_var_bit_to_var_aux_acc',
+      map_var_bit_to_var_aux_v = map_var_bit_to_var_aux_v',
+      map_var_bit_to_var_aux_n = map_var_bit_to_var_aux_n',
+      map_var_bit_to_var_aux_ret = map_var_bit_to_var_aux_ret'\<rparr>;
+    map_var_bit_to_var_aux_ret_state = 
+        map_var_bit_to_var_aux_imp map_var_bit_to_var_aux_state;
+    t = t + map_var_bit_to_var_aux_imp_time 0 map_var_bit_to_var_aux_state;
+
+    map_var_bit_to_var_acc_acc' = map_var_bit_to_var_aux_ret map_var_bit_to_var_aux_ret_state;
     t = t + 2;
-    prod_encode_ret' = 0;
-    t = t + 2;
-    prod_encode_state = \<lparr>prod_encode_a = prod_encode_a',
-                         prod_encode_b = prod_encode_b',
-      prod_encode_ret = prod_encode_ret'\<rparr>;
-    prod_encode_ret_state = prod_encode_imp prod_encode_state;
-    t = t + prod_encode_imp_time 0 prod_encode_state;
-    prod_encode_result = prod_encode_ret prod_encode_ret_state;
-    t = t + 2;
-    var_bit_to_var_nat_n' = prod_encode_result;
-    t = t + 2;
-    var_bit_to_var_nat_ret' = 0;
-    t = t + 2;
-    var_bit_to_var_nat_state = \<lparr>var_bit_to_var_nat_n = var_bit_to_var_nat_n',
-                                var_bit_to_var_nat_ret = var_bit_to_var_nat_ret'\<rparr>;
-    var_bit_to_var_nat_ret_state = var_bit_to_var_nat_imp var_bit_to_var_nat_state;
-    t = t + var_bit_to_var_nat_imp_time 0 var_bit_to_var_nat_state;
-    var_bit_to_var_nat_result = var_bit_to_var_nat_ret var_bit_to_var_nat_ret_state;
-    t = t + 2;
-    cons_h' = var_bit_to_var_nat_result;
-    t = t + 2;
-    cons_t' = map_var_bit_to_var_acc_acc s;
-    t = t + 2;
-    cons_ret' = 0;
-    t = t + 2;
-    cons_state = \<lparr>cons_h = cons_h',
-                  cons_t = cons_t', 
-                  cons_ret = cons_ret'\<rparr>;
-    cons_ret_state = cons_imp cons_state;
-    t = t + cons_imp_time 0 cons_state;
-    cons_result = cons_ret cons_ret_state;
-    t = t + 2;
-    tl_xs' = map_var_bit_to_var_acc_n s;
-    t = t + 2;
-    tl_ret' = 0;
-    t = t + 2;
-    tl_state = \<lparr>tl_xs = tl_xs', 
-                tl_ret = tl_ret'\<rparr>;
-    tl_ret_state = tl_imp tl_state;
-    t = t + tl_imp_time 0 tl_state;
-    tl_result = tl_ret tl_ret_state;
-    t = t + 2;
-    map_var_bit_to_var_acc_acc' = cons_result;
-    t = t + 2;
-    map_var_bit_to_var_acc_v' = map_var_bit_to_var_acc_v s;
-    t = t + 2;
-    map_var_bit_to_var_acc_n' = tl_result;
-    t = t + 2;
-    map_var_bit_to_var_acc_ret' = map_var_bit_to_var_acc_ret s;
+    map_var_bit_to_var_acc_n' = map_var_bit_to_var_aux_n map_var_bit_to_var_aux_ret_state;
     t = t + 2;
     ret = \<lparr>map_var_bit_to_var_acc_acc = map_var_bit_to_var_acc_acc',
-           map_var_bit_to_var_acc_v = map_var_bit_to_var_acc_v',
+           map_var_bit_to_var_acc_v = map_var_bit_to_var_acc_v s,
            map_var_bit_to_var_acc_n = map_var_bit_to_var_acc_n',
-           map_var_bit_to_var_acc_ret = map_var_bit_to_var_acc_ret'\<rparr>
+           map_var_bit_to_var_acc_ret = map_var_bit_to_var_acc_ret s\<rparr>
   in
     t
 "
@@ -239,17 +457,11 @@ definition "map_var_bit_to_var_acc_imp_compute_loop_condition_time t s \<equiv>
 
 definition "map_var_bit_to_var_acc_imp_after_loop_time t s \<equiv>
   let
-    map_var_bit_to_var_acc_acc' = map_var_bit_to_var_acc_acc s;
-    t = t + 2;
-    map_var_bit_to_var_acc_v' = map_var_bit_to_var_acc_v s;
-    t = t + 2;
-    map_var_bit_to_var_acc_n' = map_var_bit_to_var_acc_n s;
-    t = t + 2;
     map_var_bit_to_var_acc_ret' = map_var_bit_to_var_acc_acc s;
     t = t + 2;
-    ret = \<lparr>map_var_bit_to_var_acc_acc = map_var_bit_to_var_acc_acc',
-           map_var_bit_to_var_acc_v = map_var_bit_to_var_acc_v',
-           map_var_bit_to_var_acc_n = map_var_bit_to_var_acc_n',
+    ret = \<lparr>map_var_bit_to_var_acc_acc = map_var_bit_to_var_acc_acc s,
+           map_var_bit_to_var_acc_v = map_var_bit_to_var_acc_v s,
+           map_var_bit_to_var_acc_n = map_var_bit_to_var_acc_n s,
            map_var_bit_to_var_acc_ret = map_var_bit_to_var_acc_ret'\<rparr>
   in
     t
@@ -282,7 +494,8 @@ function map_var_bit_to_var_acc_imp_time::
   by auto
 termination
   apply (relation "measure (map_var_bit_to_var_acc_n \<circ> snd)")
-  by (auto simp add: map_var_bit_to_var_acc_imp_subprogram_time_simps tl_imp_correct)
+  by (auto simp add: map_var_bit_to_var_acc_imp_subprogram_time_simps
+        map_var_bit_to_var_aux_imp_correct Let_def)
 
 declare map_var_bit_to_var_acc_imp_time.simps [simp del]            
 
@@ -305,11 +518,6 @@ lemma map_var_bit_to_var_acc_imp_time_acc_3:
   by (induction a arbitrary: b s) (simp add: map_var_bit_to_var_acc_imp_time_acc)+            
 
 abbreviation "map_var_bit_to_var_acc_while_cond \<equiv> ''condition''"
-abbreviation "map_var_bit_to_var_acc_hd_result \<equiv> ''hd_result''"
-abbreviation "map_var_bit_to_var_acc_prod_encode_result \<equiv> ''prod_encode_result''"
-abbreviation "map_var_bit_to_var_acc_var_bit_to_var_nat_result \<equiv> ''var_bit_to_var_nat_result''"
-abbreviation "map_var_bit_to_var_acc_cons_result \<equiv> ''cons_result''"
-abbreviation "map_var_bit_to_var_acc_tl_result \<equiv> ''tl_result''"
 
 definition "map_var_bit_to_var_acc_IMP_init_while_cond \<equiv>
   \<comment> \<open>condition = map_var_bit_to_var_acc_n s\<close>
@@ -317,85 +525,24 @@ definition "map_var_bit_to_var_acc_IMP_init_while_cond \<equiv>
 "
 
 definition "map_var_bit_to_var_acc_IMP_loop_body \<equiv>
-  \<comment> \<open>hd_xs' = map_var_bit_to_var_acc_n s;\<close>
-  (hd_prefix @ hd_xs_str) ::= (A (V map_var_bit_to_var_acc_n_str));;
-  \<comment> \<open>hd_ret' = 0;\<close>
-  (hd_prefix @ hd_ret_str) ::= (A (N 0));;
-  \<comment> \<open>hd_state = \<lparr>hd_xs = hd_xs',\<close>
-  \<comment> \<open>            hd_ret = hd_ret'\<rparr>;\<close>
-  \<comment> \<open>hd_ret_state = hd_imp hd_state;\<close>
-  invoke_subprogram hd_prefix hd_IMP_Minus;;
-  \<comment> \<open>hd_result = hd_ret hd_ret_state;\<close>
-  map_var_bit_to_var_acc_hd_result ::= (A (V (hd_prefix @ hd_ret_str)));;
-  \<comment> \<open>prod_encode_a' = map_var_bit_to_var_acc_v s;\<close>
-  (prod_encode_prefix @ prod_encode_a_str) ::= (A (V map_var_bit_to_var_acc_v_str));;
-  \<comment> \<open>prod_encode_b' = hd_result;\<close>
-  (prod_encode_prefix @ prod_encode_b_str) ::= (A (V map_var_bit_to_var_acc_hd_result));;
-  \<comment> \<open>prod_encode_ret' = 0;\<close>
-  (prod_encode_prefix @ prod_encode_ret_str) ::= (A (N 0));;
-  \<comment> \<open>prod_encode_state = \<lparr>prod_encode_a = prod_encode_a',\<close>
-  \<comment> \<open>                     prod_encode_b = prod_encode_b',\<close>
-  \<comment> \<open>  prod_encode_ret = prod_encode_ret'\<rparr>;\<close>
-  \<comment> \<open>prod_encode_ret_state = prod_encode_imp prod_encode_state;\<close>
-  invoke_subprogram prod_encode_prefix prod_encode_IMP_Minus;;
-  \<comment> \<open>prod_encode_result = prod_encode_ret prod_encode_ret_state;\<close>
-  map_var_bit_to_var_acc_prod_encode_result ::= (A (V (prod_encode_prefix @ prod_encode_ret_str)));;
-  \<comment> \<open>var_bit_to_var_nat_n' = prod_encode_result;\<close>
-  (var_bit_to_var_nat_prefix @ var_bit_to_var_nat_n_str) ::= (A (V map_var_bit_to_var_acc_prod_encode_result));;
-  \<comment> \<open>var_bit_to_var_nat_ret' = 0;\<close>
-  (var_bit_to_var_nat_prefix @ var_bit_to_var_nat_ret_str) ::= (A (N 0));;
-  \<comment> \<open>var_bit_to_var_nat_state = \<lparr>var_bit_to_var_nat_n = var_bit_to_var_nat_n',\<close>
-  \<comment> \<open>                            var_bit_to_var_nat_ret = var_bit_to_var_nat_ret'\<rparr>;\<close>
-  \<comment> \<open>var_bit_to_var_nat_ret_state = var_bit_to_var_nat_imp var_bit_to_var_nat_state;\<close>
-  invoke_subprogram var_bit_to_var_nat_prefix var_bit_to_var_nat_IMP_Minus;;
-  \<comment> \<open>var_bit_to_var_nat_result = var_bit_to_var_nat_ret var_bit_to_var_nat_ret_state;\<close>
-  map_var_bit_to_var_acc_var_bit_to_var_nat_result ::= (A (V (var_bit_to_var_nat_prefix @ var_bit_to_var_nat_ret_str)));;
-  \<comment> \<open>cons_h' = var_bit_to_var_nat_result;\<close>
-  (cons_prefix @ cons_h_str) ::= (A (V map_var_bit_to_var_acc_var_bit_to_var_nat_result));;
-  \<comment> \<open>cons_t' = map_var_bit_to_var_acc_acc s;\<close>
-  (cons_prefix @ cons_t_str) ::= (A (V map_var_bit_to_var_acc_acc_str));;
-  \<comment> \<open>cons_ret' = 0;\<close>
-  (cons_prefix @ cons_ret_str) ::= (A (N 0));;
-  \<comment> \<open>cons_state = \<lparr>cons_h = cons_h',\<close>
-  \<comment> \<open>              cons_t = cons_t', \<close>
-  \<comment> \<open>              cons_ret = cons_ret'\<rparr>;\<close>
-  \<comment> \<open>cons_ret_state = cons_imp cons_state;\<close>
-  invoke_subprogram cons_prefix cons_IMP_Minus;;
-  \<comment> \<open>cons_result = cons_ret cons_ret_state;\<close>
-  map_var_bit_to_var_acc_cons_result ::= (A (V (cons_prefix @ cons_ret_str)));;
-  \<comment> \<open>tl_xs' = map_var_bit_to_var_acc_n s;\<close>
-  (tl_prefix @ tl_xs_str) ::= (A (V map_var_bit_to_var_acc_n_str));;
-  \<comment> \<open>tl_ret' = 0;\<close>
-  (tl_prefix @ tl_ret_str) ::= (A (N 0));;
-  \<comment> \<open>tl_state = \<lparr>tl_xs = tl_xs', \<close>
-  \<comment> \<open>            tl_ret = tl_ret'\<rparr>;\<close>
-  \<comment> \<open>tl_ret_state = tl_imp tl_state;\<close>
-  invoke_subprogram tl_prefix tl_IMP_Minus;;
-  \<comment> \<open>tl_result = tl_ret tl_ret_state;\<close>
-  map_var_bit_to_var_acc_tl_result ::= (A (V (tl_prefix @ tl_ret_str)));;
-  \<comment> \<open>map_var_bit_to_var_acc_acc' = cons_result;\<close>
-  (map_var_bit_to_var_acc_acc_str) ::= (A (V map_var_bit_to_var_acc_cons_result));;
-  \<comment> \<open>map_var_bit_to_var_acc_v' = map_var_bit_to_var_acc_v s;\<close>
-  (map_var_bit_to_var_acc_v_str) ::= (A (V map_var_bit_to_var_acc_v_str));;
-  \<comment> \<open>map_var_bit_to_var_acc_n' = tl_result;\<close>
-  (map_var_bit_to_var_acc_n_str) ::= (A (V map_var_bit_to_var_acc_tl_result));;
-  \<comment> \<open>map_var_bit_to_var_acc_ret' = map_var_bit_to_var_acc_ret s;\<close>
-  (map_var_bit_to_var_acc_ret_str) ::= (A (V map_var_bit_to_var_acc_ret_str))
-  \<comment> \<open>ret = \<lparr>map_var_bit_to_var_acc_acc = map_var_bit_to_var_acc_acc',\<close>
-  \<comment> \<open>       map_var_bit_to_var_acc_v = map_var_bit_to_var_acc_v',\<close>
-  \<comment> \<open>       map_var_bit_to_var_acc_n = map_var_bit_to_var_acc_n',\<close>
-  \<comment> \<open>       map_var_bit_to_var_acc_ret = map_var_bit_to_var_acc_ret'\<rparr>\<close>
+ (map_var_bit_to_var_aux_prefix @ map_var_bit_to_var_aux_acc_str)
+   ::= A (V map_var_bit_to_var_acc_acc_str);;
+ (map_var_bit_to_var_aux_prefix @ map_var_bit_to_var_aux_v_str)
+   ::= A (V map_var_bit_to_var_acc_v_str);;
+ (map_var_bit_to_var_aux_prefix @ map_var_bit_to_var_aux_n_str)
+   ::= A (V map_var_bit_to_var_acc_n_str);;
+ (map_var_bit_to_var_aux_prefix @ map_var_bit_to_var_aux_ret_str)
+   ::= A (N 0);;
+ invoke_subprogram map_var_bit_to_var_aux_prefix map_var_bit_to_var_aux_IMP_Minus;;
+  
+  (map_var_bit_to_var_acc_acc_str) ::= (A (V (map_var_bit_to_var_aux_prefix 
+                                             @ map_var_bit_to_var_aux_ret_str)));;
+  (map_var_bit_to_var_acc_n_str) ::=  (A (V (map_var_bit_to_var_aux_prefix 
+                                             @ map_var_bit_to_var_aux_n_str)))
 "
 
 definition "map_var_bit_to_var_acc_IMP_after_loop \<equiv>
-  \<comment> \<open>map_var_bit_to_var_acc_acc' = map_var_bit_to_var_acc_acc s;\<close>
-  (map_var_bit_to_var_acc_acc_str) ::= (A (V map_var_bit_to_var_acc_cons_result));;
-  \<comment> \<open>map_var_bit_to_var_acc_v' = map_var_bit_to_var_acc_v s;\<close>
-  (map_var_bit_to_var_acc_v_str) ::= (A (V map_var_bit_to_var_acc_v_str));;
-  \<comment> \<open>map_var_bit_to_var_acc_n' = map_var_bit_to_var_acc_n s;\<close>
-  (map_var_bit_to_var_acc_n_str) ::= (A (V map_var_bit_to_var_acc_tl_result));;
-  \<comment> \<open>map_var_bit_to_var_acc_ret' = map_var_bit_to_var_acc_acc s;\<close>
-  (map_var_bit_to_var_acc_ret_str) ::= (A (V map_var_bit_to_var_acc_cons_result))
+  (map_var_bit_to_var_acc_ret_str) ::= (A (V map_var_bit_to_var_acc_acc_str))
   \<comment> \<open>ret = \<lparr>map_var_bit_to_var_acc_acc = map_var_bit_to_var_acc_acc',\<close>
   \<comment> \<open>       map_var_bit_to_var_acc_v = map_var_bit_to_var_acc_v',\<close>
   \<comment> \<open>       map_var_bit_to_var_acc_n = map_var_bit_to_var_acc_n',\<close>
@@ -412,9 +559,9 @@ definition map_var_bit_to_var_acc_IMP_Minus where
   map_var_bit_to_var_acc_IMP_after_loop"
 
 abbreviation "map_var_bit_to_var_acc_IMP_vars\<equiv>
-  {map_var_bit_to_var_acc_while_cond, map_var_bit_to_var_acc_hd_result,
-    map_var_bit_to_var_acc_prod_encode_result, map_var_bit_to_var_acc_var_bit_to_var_nat_result,
-    map_var_bit_to_var_acc_cons_result, map_var_bit_to_var_acc_tl_result}"
+  {map_var_bit_to_var_acc_while_cond,
+    map_var_bit_to_var_acc_acc_str, map_var_bit_to_var_acc_v_str,
+  map_var_bit_to_var_acc_n_str,  map_var_bit_to_var_acc_ret_str}"
 
 lemmas map_var_bit_to_var_acc_IMP_subprogram_simps =
   map_var_bit_to_var_acc_IMP_init_while_cond_def
@@ -429,11 +576,7 @@ definition "map_var_bit_to_var_acc_imp_to_HOL_state p s =
 
 lemmas map_var_bit_to_var_acc_state_translators =
   map_var_bit_to_var_acc_imp_to_HOL_state_def
-  hd_imp_to_HOL_state_def
-  prod_encode_imp_to_HOL_state_def
-  var_bit_to_var_nat_imp_to_HOL_state_def
-  cons_imp_to_HOL_state_def
-  tl_imp_to_HOL_state_def
+  map_var_bit_to_var_aux_imp_to_HOL_state_def
 
 lemmas map_var_bit_to_var_acc_complete_simps =
   map_var_bit_to_var_acc_IMP_subprogram_simps
@@ -452,47 +595,38 @@ lemma map_var_bit_to_var_acc_IMP_Minus_correct_function:
   apply(erule Seq_E)+
   apply(erule While_tE)
 
-  sorry
-
-
-(*
-unfinished proofs by Alexander, commented incase some of them are reusable
-
-apply(simp only: map_var_bit_to_var_acc_IMP_subprogram_simps prefix_simps)
-    apply(erule Seq_E)+
-    apply(fastforce_sorted_premises2 simp: map_var_bit_to_var_acc_IMP_subprogram_simps
-        map_var_bit_to_var_acc_imp_subprogram_simps
-        map_var_bit_to_var_acc_state_translators)
+    subgoal 
+      apply (simp only: map_var_bit_to_var_acc_IMP_subprogram_simps prefix_simps)
+      apply (clarsimp simp: map_var_bit_to_var_acc_complete_simps) 
+      done 
 
   apply(erule Seq_E)+
   apply(dest_com_gen)
 
   subgoal
       apply(simp only: map_var_bit_to_var_acc_IMP_init_while_cond_def prefix_simps)
-      apply(erule Seq_E)+
-      apply(erule <?>_IMP_Minus_correct[where vars = "map_var_bit_to_var_acc_IMP_vars"])
-      subgoal premises p using p(999) by fastforce
       by(fastforce simp add: map_var_bit_to_var_acc_complete_simps)
 
   subgoal
       apply(subst (asm) map_var_bit_to_var_acc_IMP_init_while_cond_def)
       apply(simp only: map_var_bit_to_var_acc_IMP_loop_body_def prefix_simps)
       apply(erule Seq_E)+
-      apply(erule <?>_IMP_Minus_correct[where vars = "map_var_bit_to_var_acc_IMP_vars"])
-      subgoal premises p using p(999) by fastforce
-      by (simp only: map_var_bit_to_var_acc_imp_subprogram_simps
-          map_var_bit_to_var_acc_state_translators Let_def, force)
+      apply(erule map_var_bit_to_var_aux_IMP_Minus_correct[where vars = "map_var_bit_to_var_acc_IMP_vars"])
+      subgoal premises p using p(12) by fastforce
+      apply (force simp add: map_var_bit_to_var_acc_imp_subprogram_simps 
+         map_var_bit_to_var_acc_state_translators Let_def)
+      done 
 
   subgoal
       apply(simp only: map_var_bit_to_var_acc_IMP_init_while_cond_def prefix_simps
           map_var_bit_to_var_acc_IMP_loop_body_def)
       apply(erule Seq_E)+
-      apply(erule <?>_IMP_Minus_correct[where vars = "map_var_bit_to_var_acc_IMP_vars"])
-      subgoal premises p using p(999) by fastforce
-      by (simp only: map_var_bit_to_var_acc_imp_subprogram_simps
-          map_var_bit_to_var_acc_state_translators Let_def, force)
-
-*)     
+      apply(erule map_var_bit_to_var_aux_IMP_Minus_correct[where vars = "map_var_bit_to_var_acc_IMP_vars"])
+      subgoal premises p using p(12) by fastforce
+      apply (force simp add: map_var_bit_to_var_acc_imp_subprogram_simps 
+         map_var_bit_to_var_acc_state_translators Let_def split: if_splits)
+      done 
+  done 
 
 lemma map_var_bit_to_var_acc_IMP_Minus_correct_effects:
   "\<lbrakk>(invoke_subprogram (p @ map_var_bit_to_var_acc_pref) map_var_bit_to_var_acc_IMP_Minus, s) \<Rightarrow>\<^bsup>t\<^esup> s';
@@ -518,19 +652,11 @@ lemma map_var_bit_to_var_acc_IMP_Minus_correct_time:
 
   apply(erule Seq_tE)+
   apply(erule While_tE_time)
-
-  sorry 
-
-(*
-unfinished proofs by Alexander, commented incase some of them are reusable
-
-subgoal
-    apply(simp only: map_var_bit_to_var_acc_IMP_subprogram_simps prefix_simps)
-    apply(erule Seq_tE)+
-    apply(erule <?>_IMP_Minus_correct[where vars = "map_var_bit_to_var_acc_IMP_vars"])
-    subgoal premises p using p(999) by fastforce
-    by (force simp: map_var_bit_to_var_acc_IMP_subprogram_simps
-        map_var_bit_to_var_acc_imp_subprogram_time_simps map_var_bit_to_var_acc_state_translators)
+  subgoal
+    apply(simp only: map_var_bit_to_var_acc_IMP_subprogram_simps prefix_simps
+     map_var_bit_to_var_acc_complete_time_simps Let_def split: if_splits) 
+    apply force
+    done 
 
   apply(erule Seq_tE)+
   apply(simp add: add.assoc)
@@ -538,32 +664,31 @@ subgoal
 
   subgoal
     apply(simp only: map_var_bit_to_var_acc_IMP_init_while_cond_def prefix_simps)
-    apply(erule Seq_tE)+
-    apply(erule <?>_IMP_Minus_correct[where vars = "map_var_bit_to_var_acc_IMP_vars"])
-    subgoal premises p using p(999) by fastforce
     by(fastforce simp add: map_var_bit_to_var_acc_complete_simps)
 
   subgoal
     apply(subst (asm) map_var_bit_to_var_acc_IMP_init_while_cond_def)
     apply(simp only: map_var_bit_to_var_acc_IMP_loop_body_def prefix_simps)
     apply(erule Seq_tE)+
-    apply(erule <?>_IMP_Minus_correct[where vars = "map_var_bit_to_var_acc_IMP_vars"])
-    subgoal premises p using p(999) by fastforce
-    by (simp only: map_var_bit_to_var_acc_imp_subprogram_time_simps
-        map_var_bit_to_var_acc_state_translators Let_def, force)
+    apply(erule map_var_bit_to_var_aux_IMP_Minus_correct[where vars = "map_var_bit_to_var_acc_IMP_vars"])
+    subgoal premises p using p(21) by fastforce
+    apply (force simp: map_var_bit_to_var_acc_imp_subprogram_time_simps
+        map_var_bit_to_var_acc_state_translators Let_def)
+    done 
 
   subgoal
     apply(simp only: prefix_simps map_var_bit_to_var_acc_IMP_init_while_cond_def
         map_var_bit_to_var_acc_IMP_loop_body_def)
     apply(erule Seq_tE)+
-    apply(erule <?>_IMP_Minus_correct[where vars = "map_var_bit_to_var_acc_IMP_vars"])
-    subgoal premises p using p(999) by fastforce
-    apply(simp only: map_var_bit_to_var_acc_complete_time_simps Let_def)
-    by force
-
-  done      
-
-*) 
+    apply(erule map_var_bit_to_var_aux_IMP_Minus_correct[where vars = "map_var_bit_to_var_acc_IMP_vars"])
+    subgoal premises p using p(21) by fastforce
+    apply (clarsimp simp add: map_var_bit_to_var_acc_complete_time_simps Let_def)
+    subgoal premises p 
+      using p(10) 
+      by (smt (z3) fun_upd_def list.inject list.simps(3) 
+      map_var_bit_to_var_acc_imp_time_acc_2_aux same_append_eq)
+    done  
+  done   
 
 lemma map_var_bit_to_var_acc_IMP_Minus_correct[functional_correctness]:
   "\<lbrakk>(invoke_subprogram (p1 @ p2) map_var_bit_to_var_acc_IMP_Minus, s) \<Rightarrow>\<^bsup>t\<^esup> s';
@@ -730,7 +855,7 @@ lemma push_on_stack_nat_eq_zero_IMP_Minus_correct_function:
    subgoal premises p using p(15) by fastforce 
    apply (erule cons_IMP_Minus_correct[where vars=push_on_stack_nat_IMP_vars])
    subgoal premises p using p(17) by fastforce 
-   apply (force simp: push_on_stack_nat_eq_zero_def
+   apply (force simp: 
       push_on_stack_nat_imp_to_HOL_state_def cons_imp_to_HOL_state_def Let_def)
    done 
 
@@ -746,7 +871,7 @@ lemma push_on_stack_nat_eq_zero_IMP_Minus_correct_time:
    subgoal premises p using p(27) by fastforce 
    apply (erule cons_IMP_Minus_correct[where vars=push_on_stack_nat_IMP_vars])
    subgoal premises p using p(29) by fastforce 
-   apply (timeit \<open>force simp: push_on_stack_nat_eq_zero_time_def
+   apply (timeit \<open>force simp:
       push_on_stack_nat_imp_to_HOL_state_def cons_imp_to_HOL_state_def Let_def\<close>)
    done
 
@@ -965,7 +1090,7 @@ lemma push_on_stack_nat_eq_one_IMP_Minus_correct_function:
    subgoal premises p using p(41) by fastforce 
    apply (erule cons_IMP_Minus_correct[where vars=push_on_stack_nat_IMP_vars_eq_one])
    subgoal premises p using p(43) by fastforce
-   apply (timeit \<open>force simp: push_on_stack_nat_eq_one_def
+   apply (timeit \<open>force simp:
       push_on_stack_nat_imp_to_HOL_state_def cons_imp_to_HOL_state_def 
       nth_nat_imp_to_HOL_state_def Let_def\<close>)
    done
@@ -991,7 +1116,7 @@ lemma push_on_stack_nat_eq_one_IMP_Minus_correct_time:
   subgoal premises p using p(71) by fastforce 
   apply (erule cons_IMP_Minus_correct[where vars=push_on_stack_nat_IMP_vars_eq_one])
   subgoal premises p using p(73) by fastforce
-  apply (timeit \<open>force simp: push_on_stack_nat_eq_one_time_def
+  apply (timeit \<open>force simp: 
       push_on_stack_nat_imp_to_HOL_state_def cons_imp_to_HOL_state_def 
       nth_nat_imp_to_HOL_state_def Let_def\<close>)
   done
@@ -1211,7 +1336,7 @@ lemma push_on_stack_nat_eq_two_IMP_Minus_correct_function:
    subgoal premises p using p(41) by fastforce 
    apply (erule cons_IMP_Minus_correct[where vars=push_on_stack_nat_IMP_vars_eq_two])
    subgoal premises p using p(43) by fastforce
-   apply (timeit \<open>force simp: push_on_stack_nat_eq_two_def
+   apply (timeit \<open>force simp:
       push_on_stack_nat_imp_to_HOL_state_def cons_imp_to_HOL_state_def 
       nth_nat_imp_to_HOL_state_def Let_def\<close>)
    done
@@ -1236,7 +1361,7 @@ lemma push_on_stack_nat_eq_two_IMP_Minus_correct_time:
   subgoal premises p using p(71) by fastforce 
   apply (erule cons_IMP_Minus_correct[where vars=push_on_stack_nat_IMP_vars_eq_two])
   subgoal premises p using p(73) by fastforce
-  apply (timeit \<open>force simp: push_on_stack_nat_eq_two_time_def
+  apply (timeit \<open>force simp:
       push_on_stack_nat_imp_to_HOL_state_def cons_imp_to_HOL_state_def 
       nth_nat_imp_to_HOL_state_def Let_def\<close>)
   done
@@ -1456,7 +1581,7 @@ lemma push_on_stack_nat_else_IMP_Minus_correct_function:
    subgoal premises p using p(41) by fastforce 
    apply (erule cons_IMP_Minus_correct[where vars=push_on_stack_nat_IMP_vars_else])
    subgoal premises p using p(43) by fastforce
-   apply (timeit \<open>force simp: push_on_stack_nat_else_def
+   apply (timeit \<open>force simp:
       push_on_stack_nat_imp_to_HOL_state_def cons_imp_to_HOL_state_def 
       nth_nat_imp_to_HOL_state_def Let_def\<close>)
    done
@@ -1482,7 +1607,7 @@ lemma push_on_stack_nat_else_IMP_Minus_correct_time:
   subgoal premises p using p(71) by fastforce 
   apply (erule cons_IMP_Minus_correct[where vars=push_on_stack_nat_IMP_vars_else])
   subgoal premises p using p(73) by fastforce
-  apply (timeit \<open>force simp: push_on_stack_nat_else_time_def
+  apply (timeit \<open>force simp:
       push_on_stack_nat_imp_to_HOL_state_def cons_imp_to_HOL_state_def 
       nth_nat_imp_to_HOL_state_def Let_def\<close>)
   done
@@ -1754,7 +1879,7 @@ lemma push_on_stack_nat_eq_three_IMP_Minus_correct_function:
    subgoal premises p using p(54) by fastforce
    apply (erule cons_IMP_Minus_correct[where vars=push_on_stack_nat_IMP_vars_eq_three])
    subgoal premises p using p(56) by fastforce
-   apply (timeit \<open>force simp: push_on_stack_nat_eq_three_def
+   apply (timeit \<open>force simp:
       push_on_stack_nat_imp_to_HOL_state_def cons_imp_to_HOL_state_def 
       nth_nat_imp_to_HOL_state_def Let_def\<close>)
    done 
@@ -1784,7 +1909,7 @@ lemma push_on_stack_nat_eq_three_IMP_Minus_correct_time:
    subgoal premises p using p(93) by fastforce
    apply (erule cons_IMP_Minus_correct[where vars=push_on_stack_nat_IMP_vars_eq_three])
    subgoal premises p using p(95) by fastforce
-  apply (force simp: push_on_stack_nat_eq_three_time_def
+  apply (force simp: 
       push_on_stack_nat_imp_to_HOL_state_def cons_imp_to_HOL_state_def 
       nth_nat_imp_to_HOL_state_def Let_def)
   done
